src/proof/controllers/statefulset/outdated.v
@@ -1,0 +1,290 @@
+From New.proof Require Import prelude empty_ffi.
+From New.proof.controllers.statefulset Require Export pod_predicates.
+
+Section proof.
+Context `{hG: !heapGS Σ} `{!ffi_semantics _ _}.
+Context {sem : go.Semantics}
+  {package_sem : code.controllers.statefulset.statefulset.Assumptions}.
+Collection W := sem + package_sem.
+#[local] Instance base_common_sem : common.Assumptions | 100 :=
+  code.controllers.statefulset.statefulset.import_common_Assumption.
+#[local] Instance controller_sem : controller.Assumptions :=
+  code.controllers.statefulset.statefulset.import_controller_Assumption.
+#[local] Instance runtime_sem : code.k8s_io.apimachinery.pkg.runtime.runtime.Assumptions :=
+  controller.import_runtime_Assumption.
+#[local] Instance runtime_object_underlying_eq :
+    runtime.Object ≤u runtime.Objectⁱᵐᵖˡ.
+Proof using package_sem. apply _. Qed.
+#[local] Instance meta_object_underlying_eq :
+    meta_v1.Object ≤u meta_v1.Objectⁱᵐᵖˡ.
+Proof using package_sem. apply _. Qed.
+#[local] Instance base_apimodel_sem : apimodel.Assumptions | 100 :=
+  common.import_apimodel_Assumption.
+#[local] Instance object_meta_v1_sem :
+    code.k8s_io.apimachinery.pkg.apis.meta.v1.v1.Assumptions :=
+  apimodel.import_apis_meta_v1_Assumption.
+#[local] Instance object_apps_v1_sem :
+    code.k8s_io.api.apps.v1.v1.Assumptions :=
+  apimodel.import_api_apps_v1_Assumption.
+#[local] Instance object_core_v1_sem :
+    code.k8s_io.api.core.v1.v1.Assumptions :=
+  code.k8s_io.api.apps.v1.v1.import_core_v1_Assumption.
+#[local] Instance apimodel_sem : apimodel.Assumptions | 0.
+Proof using package_sem.
+  constructor; try exact object_core_v1_sem; try apply _.
+Defined.
+#[local] Instance common_sem : common.Assumptions | 0.
+Proof using package_sem.
+  constructor; try exact apimodel_sem; try apply _.
+Defined.
+Context `{!kubernetesModelG Σ}.
+Local Set Default Proof Using "All".
+
+Definition pod_is_outdated (set : StatefulSetV.t) (pod : PodV.t) : Prop :=
+  ∃ ordinal,
+    (ordinal ≤ go_int32_max_nat)%nat ∧
+    pod.(PodV.ObjectMeta').(ObjectMetaV.Name') =
+      desired_pod_name
+        set.(StatefulSetV.ObjectMeta').(ObjectMetaV.Name') ordinal ∧
+    (ordinal < statefulset_replicas set)%nat ∧
+    ¬ pod_immutable_matches set pod.
+
+Lemma wp_withoutStatefulSetFields
+    (spec_c : v1.PodSpec.t) (spec : PodSpecV.t) dq :
+  {{{ PodSpecV.deepown spec_c spec dq }}}
+    @! statefulset.withoutStatefulSetFields #spec_c
+  {{{ result_c, RET #result_c;
+      PodSpecV.deepown spec_c spec dq ∗
+      PodSpecV.deepown result_c (without_statefulset_fields spec) dq
+  }}}.
+Proof.
+  wp_start as "Hspec".
+  iNamed "Hspec".
+  wp_auto.
+  iApply "HΦ".
+  iSplitL "Hdeepown_volumes".
+  - rewrite /PodSpecV.deepown. iFrame. done.
+  - rewrite /PodSpecV.deepown /without_statefulset_fields /=.
+    iSplitL.
+    + iExists []. rewrite /deepown_list big_sepL2_nil.
+      iSplit; [iApply own_slice_nil|done].
+    + done.
+Qed.
+
+Lemma wp_podSpecMatches set_l pod_l
+    (set : StatefulSetV.t) (pod : PodV.t) dq_set dq_pod :
+  {{{ StatefulSetV.deepown_l set_l set dq_set ∗
+      PodV.deepown_l pod_l pod dq_pod
+  }}}
+    @! statefulset.podSpecMatches #set_l #pod_l
+  {{{ (ret : bool), RET #ret;
+      ⌜ ret = true ↔ pod_immutable_matches set pod ⌝ ∗
+      StatefulSetV.deepown_l set_l set dq_set ∗
+      PodV.deepown_l pod_l pod dq_pod
+  }}}.
+Proof. Admitted.
+
+Lemma wp_largestOutdatedPod set_l pods_sl
+    (set : StatefulSetV.t) (ptrs : list loc) (pods : list PodV.t)
+    dq_set dq_pods :
+  {{{ "Hset" ∷ StatefulSetV.deepown_l set_l set dq_set ∗
+      "Hpods_sl" ∷ pods_sl ↦* ptrs ∗
+      "Hpods" ∷ ([∗ list] ptr;pod ∈ ptrs;pods,
+        PodV.deepown_l ptr pod dq_pods) ∗
+      "%Hspec_valid" ∷ ⌜ StatefulSetSpecV.valid set.(StatefulSetV.Spec') ⌝ ∗
+      "%Hpod_name_len" ∷ ⌜ Forall (λ pod,
+        Z.of_nat (length pod.(PodV.ObjectMeta').(ObjectMetaV.Name')) ≤
+          go_int_max) pods ⌝ ∗
+      "%Hpods_members" ∷ ⌜ Forall (λ pod,
+        pod_has_int32_member_name
+          set.(StatefulSetV.ObjectMeta').(ObjectMetaV.Name')
+          pod.(PodV.ObjectMeta').(ObjectMetaV.Name')) pods ⌝ ∗
+      "%Hpod_names_nodup" ∷ ⌜ NoDup
+        ((λ pod, pod.(PodV.ObjectMeta').(ObjectMetaV.Name')) <$> pods) ⌝
+  }}}
+    @! statefulset.largestOutdatedPod #set_l #pods_sl
+  {{{ outdated_l, RET #outdated_l;
+      StatefulSetV.deepown_l set_l set dq_set ∗
+      pods_sl ↦* ptrs ∗
+      ([∗ list] ptr;pod ∈ ptrs;pods,
+        PodV.deepown_l ptr pod dq_pods) ∗
+      ⌜ (outdated_l = null ∧
+          Forall (λ pod, ¬ pod_is_outdated set pod) pods) ∨
+        (∃ idx pod,
+          ptrs !! idx = Some outdated_l ∧
+          pods !! idx = Some pod ∧
+          pod_is_outdated set pod) ⌝
+  }}}.
+Proof.
+  wp_start as "H". iNamed "H".
+  assert (∀ pod, pod ∈ pods →
+      Z.of_nat (length pod.(PodV.ObjectMeta').(ObjectMetaV.Name')) ≤
+        go_int_max) as Hpod_name_len_lookup.
+  { rewrite Forall_forall in Hpod_name_len.
+    intros pod' Hpod'. apply Hpod_name_len.
+    by rewrite -list_elem_of_In. }
+  wp_auto.
+  wp_apply (wp_endOrdinalOf with "[$Hset //]").
+  iIntros (end_ordinal) "[%Hend_ordinal Hset]".
+  wp_auto.
+  pose proof (StatefulSetSpecV.valid_replicas _ Hspec_valid) as
+    (replicas32 & Hreplicas & Hreplicas_nonnegative).
+  assert ((statefulset_replicas set ≤ go_int32_max_nat)%nat) as
+    Hreplicas_bound.
+  { rewrite /statefulset_replicas Hreplicas /go_int32_max_nat.
+    apply Z2Nat.inj_le.
+    - exact Hreplicas_nonnegative.
+    - unfold go_int32_max.
+      assert (0 < (2 : Z) ^ 31) by
+        (apply Z.pow_pos_nonneg; lia).
+      lia.
+    - unfold go_int32_max.
+      pose proof (word.signed_range replicas32).
+      lia. }
+  set I := (∃ (i : w64),
+    "Hi_ptr" ∷ ordinal_ptr ↦ i ∗
+    "Hset_ptr" ∷ set_ptr ↦ set_l ∗
+    "Hset" ∷ StatefulSetV.deepown_l set_l set dq_set ∗
+    "Hpods" ∷ ([∗ list] ptr;pod ∈ ptrs;pods,
+      PodV.deepown_l ptr pod dq_pods) ∗
+    "%Hi_upper" ∷ ⌜ sint.Z i ≤
+      Z.of_nat (statefulset_replicas set) - 1 ⌝ ∗
+    "%Hremaining" ∷ ⌜ ∀ pod ordinal,
+      pod ∈ pods →
+      (ordinal ≤ go_int32_max_nat)%nat →
+      pod.(PodV.ObjectMeta').(ObjectMetaV.Name') =
+        desired_pod_name
+          set.(StatefulSetV.ObjectMeta').(ObjectMetaV.Name') ordinal →
+      (ordinal < statefulset_replicas set)%nat →
+      ¬ pod_immutable_matches set pod →
+      Z.of_nat ordinal ≤ sint.Z i ⌝
+  )%I.
+  iAssert I with "[ordinal set Hset Hpods]" as "Hloop_inv".
+  { iExists end_ordinal. iFrame.
+    iPureIntro. split; [lia|].
+    intros pod' ordinal' Hpod' _ _ Hordinal' _.
+    lia. }
+  wp_for "Hloop_inv". wp_if_destruct.
+  - assert (0 ≤ sint.Z i) as Hi_nonnegative by word.
+    assert ((sint.nat i ≤ statefulset_replicas set)%nat) as
+      Hi_replicas_bound.
+    { rewrite -(Nat2Z.id (statefulset_replicas set)).
+      apply (proj1 (Z2Nat.inj_le
+        (sint.Z i) (Z.of_nat (statefulset_replicas set))
+        Hi_nonnegative ltac:(lia))).
+      lia. }
+    assert ((sint.nat i ≤ go_int32_max_nat)%nat) as
+      Hi_int32_bound by lia.
+    wp_apply (wp_findPodByOrdinal with
+      "[$Hset $Hpods_sl $Hpods]").
+    { iPureIntro. split.
+      - split.
+        + exact Hi_nonnegative.
+        + exact Hi_int32_bound.
+      - split; [exact Hpod_name_len_lookup|exact Hpods_members]. }
+    iIntros (found_l) "(Hset & Hpods_sl & Hpods & %Hfound)".
+    wp_auto.
+    destruct (find_pod_by_ordinal
+      set.(StatefulSetV.ObjectMeta').(ObjectMetaV.Name')
+      (sint.nat i) pods) as [[found_idx found_pod]|] eqn:Hfind.
+    + apply list_find_Some in Hfind as
+        (Hfound_pod_lookup & Hfound_name & _).
+      iDestruct (big_sepL2_lookup_acc with "Hpods") as
+        "[Hfound_pod Hpods_restore]";
+        [exact Hfound|exact Hfound_pod_lookup|].
+      iPoseProof (PodV.deepown_l_split with "Hfound_pod") as
+        "(%Hfound_l_not_null & Hfound_typemeta & Hfound_objectmeta & Hfound_spec & Hfound_status)".
+      iPoseProof (PodV.deepown_l_restore _ _ _ Hfound_l_not_null with
+        "[$Hfound_typemeta $Hfound_objectmeta $Hfound_spec $Hfound_status]")
+        as "Hfound_pod".
+      replace (bool_decide (found_l = null)) with false by
+        (symmetry; apply bool_decide_eq_false_2; done).
+      wp_auto.
+      wp_apply (wp_podSpecMatches with "[$Hset $Hfound_pod]").
+      iIntros (matches) "(%Hmatches & Hset & Hfound_pod)".
+      iSpecialize ("Hpods_restore" with "Hfound_pod").
+      iRename "Hpods_restore" into "Hpods".
+      destruct matches.
+      * wp_auto.
+        replace (bool_decide true) with true by done.
+        iApply wp_for_post_do. wp_auto.
+        iFrame "pods Hpods_sl HΦ".
+        iExists (word.sub i (W64 1)).
+        iFrame.
+        iPureIntro. split; [word|].
+        intros pod' ordinal' Hpod' Hordinal_bound Hpod_name
+          Hordinal_range Hnot_matches.
+        specialize (Hremaining pod' ordinal' Hpod' Hordinal_bound
+          Hpod_name Hordinal_range Hnot_matches).
+        destruct (decide (Z.of_nat ordinal' = sint.Z i)) as
+          [Hordinal_eq|Hordinal_ne].
+        -- assert (ordinal' = sint.nat i) as ->.
+           { apply Nat2Z.inj. rewrite Hordinal_eq. word. }
+           assert (∃ pod_idx, pods !! pod_idx = Some pod') as
+             [pod_idx Hpod_lookup].
+           { apply list_elem_of_lookup_1. exact Hpod'. }
+           assert (pod_idx = found_idx) as ->.
+           { apply (NoDup_lookup
+               ((λ pod,
+                 pod.(PodV.ObjectMeta').(ObjectMetaV.Name')) <$> pods)
+               pod_idx found_idx
+               (desired_pod_name
+                 set.(StatefulSetV.ObjectMeta').(ObjectMetaV.Name')
+                 (sint.nat i)) Hpod_names_nodup).
+             - rewrite list_lookup_fmap Hpod_lookup /=.
+               f_equal. exact Hpod_name.
+             - rewrite list_lookup_fmap Hfound_pod_lookup /=.
+               f_equal. exact Hfound_name. }
+           rewrite Hfound_pod_lookup in Hpod_lookup. simplify_eq/=.
+        -- word.
+      * wp_auto.
+        replace (bool_decide false) with false by done.
+        iApply wp_for_post_return. wp_auto.
+        iApply ("HΦ" $! found_l). iFrame.
+        iPureIntro. right.
+        exists found_idx, found_pod. repeat split; try done.
+        exists (sint.nat i). split.
+        -- exact Hi_int32_bound.
+        -- split; [exact Hfound_name|].
+           split.
+           ++ replace (Z.of_nat (sint.nat i)) with (sint.Z i) by word.
+              lia.
+           ++ intros Himmutable.
+              pose proof (proj2 Hmatches Himmutable).
+              done.
+    + subst found_l.
+      wp_auto.
+      replace (bool_decide (null = null)) with true by
+        (symmetry; apply bool_decide_eq_true_2; done).
+      iApply wp_for_post_do. wp_auto.
+      iFrame "pods Hpods_sl HΦ".
+      iExists (word.sub i (W64 1)).
+      iFrame.
+      iPureIntro. split; [word|].
+      intros pod' ordinal' Hpod' Hordinal_bound Hpod_name
+        Hordinal_range Hnot_matches.
+      specialize (Hremaining pod' ordinal' Hpod' Hordinal_bound
+        Hpod_name Hordinal_range Hnot_matches).
+      destruct (decide (Z.of_nat ordinal' = sint.Z i)) as
+        [Hordinal_eq|Hordinal_ne].
+      * assert (ordinal' = sint.nat i) as ->.
+        { apply Nat2Z.inj. rewrite Hordinal_eq. word. }
+        apply list_find_None in Hfind.
+        rewrite Forall_forall in Hfind.
+        exfalso. apply (Hfind pod').
+        { by rewrite -list_elem_of_In. }
+        exact Hpod_name.
+      * word.
+  - iApply ("HΦ" $! null). iFrame.
+    iPureIntro. left. split; [done|].
+    apply Forall_forall. intros pod' Hpod' Houtdated.
+    destruct Houtdated as
+      (ordinal' & Hordinal_bound & Hpod_name &
+        Hordinal_range & Hnot_matches).
+    rewrite -list_elem_of_In in Hpod'.
+    specialize (Hremaining pod' ordinal' Hpod' Hordinal_bound
+      Hpod_name Hordinal_range Hnot_matches).
+    word.
+Qed.
+
+End proof.
